Organize with Modules

theories/stlc.v
@@ -14,190 +14,153 @@ Import ListNotations.
 
 (** *** Types *)
 
-Inductive ty : Set :=
-  | ty_proposition : ty
-  | ty_individual : ty
-  | ty_arrow : ty -> ty -> ty.
+(** Interface for the types of stlc.  There must be a type for propositions and
+    an arrow type. *)
+Module Type TY.
+  Parameter ty : Set.
+  Parameter ty_prp : ty.
+  Parameter ty_arr : ty -> ty -> ty.
+End TY.
 
-(** Notations *)
-
+(** Global notation declarations. *)
 Declare Scope stlc_scope.
 Delimit Scope stlc_scope with stlc.
 Open Scope stlc_scope.
 Declare Custom Entry stlc_ty.
 
-Notation "<[ x ]>" := x (x custom stlc_ty) : stlc_scope.
-Notation "x" := x (in custom stlc_ty at level 0, x global) : stlc_scope.
-Notation "( t )" := t
-  (in custom stlc_ty at level 0, t custom stlc_ty) : stlc_scope.
-Notation "A -> B" := (ty_arrow A B)
-  (in custom stlc_ty at level 99, right associativity) : stlc_scope.
-Notation "'o'" := ty_proposition (in custom stlc_ty at level 0) : stlc_scope.
-Notation "'i'" := ty_individual (in custom stlc_ty at level 0) : stlc_scope.
+Module TyTheories (Ty : TY).
+  Export Ty.
 
-(** Examples *)
-Check <[ o ]>.
-Check <[ o -> i ]>.
-Check <[ o -> (i -> o) ]>.
-Check <[ (o -> i) -> o ]>.
+  Definition context := list ty.
+
+  Notation "<[ x ]>" := x (x custom stlc_ty) : stlc_scope.
+  Notation "x" := x (in custom stlc_ty at level 0, x global) : stlc_scope.
+  Notation "A -> B" := (ty_arr A B)
+    (in custom stlc_ty at level 99, right associativity) : stlc_scope.
+  Notation "( t )" := t
+    (in custom stlc_ty at level 0, t custom stlc_ty) : stlc_scope.
+  Notation "'o'" := ty_prp (in custom stlc_ty at level 0) : stlc_scope.
+End TyTheories.
+
+Module TyChurch <: TY.
+  Inductive tyc : Set :=
+    | tyc_prp : tyc
+    | tyc_obj : tyc
+    | tyc_arr : tyc -> tyc -> tyc.
+
+  Definition ty := tyc.
+  Definition ty_prp := tyc_prp.
+  Definition ty_arr := tyc_arr.
+End TyChurch.
+
+Module TyChurchTheories.
+  Module TyTheories := TyTheories TyChurch.
+  Import TyTheories.
+
+  Notation "'i'" := tyc_obj (in custom stlc_ty at level 0) : stlc_scope.
+
+  (** Examples *)
+  Check <[ o ]>.
+  Check <[ o -> i ]>.
+  Check <[ o -> (i -> o) ]>.
+  Check <[ (o -> i) -> o ]>.
+End TyChurchTheories.
 
 
 (** *** Terms *)
 
-(** Terms using de Bruijn levels *)
-Inductive tm : Set :=
-  | tm_lvl : nat -> tm
-  | tm_app : tm -> tm -> tm
-  | tm_abs : ty -> tm -> tm
-  | tm_bot : tm
-  | tm_top : tm
-  | tm_and : tm
-  | tm_or  : tm
-  | tm_imp : tm
-  | tm_for : ty -> tm
-  | tm_ex  : ty -> tm.
-
-(** Notations *)
-
 Declare Custom Entry stlc_tm.
 
-Notation "<{ x }>" := x (x custom stlc_tm at level 200) : stlc_scope.
-Notation "x" := x
-  (in custom stlc_tm at level 0, x constr at level 0) : stlc_scope.
-Notation "( t )" := t
-  (in custom stlc_tm at level 0, t custom stlc_tm) : stlc_scope.
-Notation "$( x )" := x
-  (in custom stlc_tm at level 0, x constr, only parsing) : stlc_scope.
-Notation "x y" := (tm_app x y)
-  (in custom stlc_tm at level 10, left associativity) : stlc_scope.
-Notation "\: A , t" := (tm_abs A t)
-  (in custom stlc_tm at level 200, A custom stlc_ty,
-  t custom stlc_tm at level 200, left associativity) : stlc_scope.
-Notation "_|" := (tm_bot)
-  (in custom stlc_tm at level 0) : stlc_scope.
-Notation "^|" := (tm_top)
-  (in custom stlc_tm at level 0) : stlc_scope.
-Notation "x /\ y" := (tm_and x y)
-  (in custom stlc_tm at level 50, left associativity) : stlc_scope.
-Notation "x \/ y" := (tm_or x y)
-  (in custom stlc_tm at level 60, left associativity) : stlc_scope.
-Notation "x > y" := (tm_imp x y)
-  (in custom stlc_tm at level 70, left associativity) : stlc_scope.
-Coercion tm_lvl : nat >-> tm.
+Module Stlc (Ty : TY).
+  Module TyTheories := TyTheories Ty.
+  Export TyTheories.
 
-(** Examples *)
-Check <{ \: i, 0 }>.
-Check <{ (\: (i -> o), 2) 1 }>.
-Check <{ \: o, 3 _| }>.
+  (** Terms using de Bruijn levels *)
+  Inductive tm : Set :=
+    | tm_lvl : nat -> tm
+    | tm_app : tm -> tm -> tm
+    | tm_abs : ty -> tm -> tm
+    | tm_bot : tm
+    | tm_top : tm
+    | tm_and : tm
+    | tm_or  : tm
+    | tm_imp : tm
+    | tm_for : ty -> tm
+    | tm_ex  : ty -> tm.
+  Check tm_rec.
 
+  (** Notations *)
+  Notation "<{ x }>" := x (x custom stlc_tm at level 200) : stlc_scope.
+  Notation "x" := x
+    (in custom stlc_tm at level 0, x constr at level 0) : stlc_scope.
+  Notation "( t )" := t
+    (in custom stlc_tm at level 0, t custom stlc_tm) : stlc_scope.
+  Notation "$( x )" := x
+    (in custom stlc_tm at level 0, x constr, only parsing) : stlc_scope.
+  Notation "x y" := (tm_app x y)
+    (in custom stlc_tm at level 10, left associativity) : stlc_scope.
+  Notation "\: A , t" := (tm_abs A t)
+    (in custom stlc_tm at level 200, A custom stlc_ty,
+    t custom stlc_tm at level 200, left associativity) : stlc_scope.
+  Notation "_|" := (tm_bot)
+    (in custom stlc_tm at level 0) : stlc_scope.
+  Notation "^|" := (tm_top)
+    (in custom stlc_tm at level 0) : stlc_scope.
+  Notation "x /\ y" := (tm_and x y)
+    (in custom stlc_tm at level 50, left associativity) : stlc_scope.
+  Notation "x \/ y" := (tm_or x y)
+    (in custom stlc_tm at level 60, left associativity) : stlc_scope.
+  Notation "x > y" := (tm_imp x y)
+    (in custom stlc_tm at level 70, left associativity) : stlc_scope.
+  Coercion tm_lvl : nat >-> tm.
 
-(**************)
-(** ** Typing *)
-(**************)
-
-Inductive has_type : list ty -> tm -> ty -> Prop :=
-  | T_Var : forall gam x T, nth_error gam x = Some T -> has_type gam x T
-  | T_Abs : forall gam T1 T2 t1,
-      has_type (gam ++ [T2]) t1 T1 ->
-      has_type gam <{ \: T2, t1 }> <[ T2 -> T1 ]>
-  | T_App : forall T1 T2 gam t1 t2,
-      has_type gam t1 <[ T2 -> T1 ]> ->
-      has_type gam t2 T2 ->
-      has_type gam <{ t1 t2 }> T1
-  | T_Bot gam : has_type gam tm_bot ty_proposition
-  | T_Top gam : has_type gam tm_top ty_proposition
-  | T_And gam :
-      has_type gam tm_and <[ o -> o -> o ]>
-  | T_Or gam :
-      has_type gam tm_or <[ o -> o -> o ]>
-  | T_Imp gam :
-      has_type gam tm_imp <[ o -> o -> o ]>
-  | T_For gam T :
-      has_type gam (tm_for T) <[ (T -> o) -> o ]>
-  | T_Ex gam T :
-      has_type gam (tm_ex T) <[ (T -> o) -> o ]>.
-
-(** Notations *)
-
-Infix "++" := app
-  (in custom stlc_ty at level 60, right associativity) : stlc_scope.
-Infix "::" := cons (in custom stlc_ty at level 60, right associativity) : stlc_scope.
-Notation "[ ]" := nil (in custom stlc_ty, format "[ ]") : stlc_scope.
-Notation "[ x ]" := (cons x nil) (in custom stlc_ty) : stlc_scope.
-Notation "[ x ; y ; .. ; z ]" := (cons x (cons y .. (cons z nil) ..))
-  (in custom stlc_ty,
-  format "[ '[' x ;  '/' y ;  '/' .. ;  '/' z ']' ]") : stlc_scope.
-
-Notation "<| gam |- t : T |>" := (has_type gam t T)
-  (at level 0, gam custom stlc_ty at level 200,
-  t custom stlc_tm, T custom stlc_ty) : stlc_scope.
-(*Notation "<| |- t : T |>" := (has_type nil t T)
-  (at level 0, t custom stlc_tm, T custom stlc_ty) : stlc_scope.*)
-
-(** Examples *)
-
-Theorem ex1 : <| [i; o] |- 0 : i |>.
-Proof. now apply T_Var. Qed.
-
-Theorem ex2 : <| [i; o] |- 1 : o |>.
-Proof. now apply T_Var. Qed.
-
-Theorem ex3 : <| [] |- \: i -> o, \: i, 0 1 : (i -> o) -> i -> o |>.
-Proof.
-  apply T_Abs. simpl. apply T_Abs. simpl.
-  eapply T_App.
-  - apply T_Var. simpl. reflexivity.
-  - apply T_Var. simpl. reflexivity.
-Qed.
-
-Theorem ex4 : <| [] |- \: i, _| : i -> o |>.
-Proof.  apply T_Abs. simpl. apply T_Bot. Qed.
-
-Theorem ex5 : forall T, ~ <| [] |- \: i, 1 : T |>.
-Proof.
-  intros T P.
-  inversion P. simpl in *. subst.
-  inversion H3. simpl in *. subst. discriminate.
-Qed.
+  (** Examples *)
+  Check fun x : ty => <{ \: x, 0 }>.
+  Check fun x : ty => <{ (\: (x -> o), 2) 1 }>.
+  Check <{ \: o, 3 _| }>.
 
 
-(********************)
-(** ** Substitution *)
-(********************)
+  (**************)
+  (** ** Typing *)
+  (**************)
 
-Notation "[ x ]" := (cons x nil) (in custom stlc_tm) : stlc_scope.
-Notation "[ x ; y ; .. ; z ]" := (cons x (cons y .. (cons z nil) ..))
-  (in custom stlc_tm,
-  format "[ '[' x ;  '/' y ;  '/' .. ;  '/' z ']' ]") : stlc_scope.
+  Inductive has_type : context -> tm -> ty -> Prop :=
+    | t_lvl c n T : nth_error c n = Some T -> has_type c n T
+    | t_abs c A B t : has_type (c ++ [A]) t B ->
+        has_type c (tm_abs A t) (ty_arr A B)
+    | t_app c A B s t : has_type c s (ty_arr A B) -> has_type c t A ->
+        has_type c (tm_app s t) B
+    | t_bot c : has_type c tm_bot ty_prp
+    | t_top c : has_type c tm_top ty_prp
+    | t_and c : has_type c tm_and <[ o -> o -> o ]>
+    | t_or  c : has_type c tm_or  <[ o -> o -> o ]>
+    | t_imp c : has_type c tm_imp <[ o -> o -> o ]>
+    | t_for c T : has_type c (tm_for T) <[ (T -> o) -> o ]>
+    | t_ex  c T : has_type c (tm_ex  T) <[ (T -> o) -> o ]>.
 
-(** Increase the levels in a term by 1 *)
-Fixpoint incr m (t : tm) : tm :=
-  match t with
-  | tm_lvl n => tm_lvl (if Nat.leb m n then S n else n)
-  | tm_app t1 t2 => tm_app (incr m t1) (incr m t2)
-  | tm_abs T t1 => tm_abs T (incr m t1)
-  | x => x
-  end.
+  Notation "<| gam |- t : T |>" := (has_type gam t T)
+    (at level 0, gam custom stlc_ty at level 200,
+    t custom stlc_tm, T custom stlc_ty) : stlc_scope.
 
-Reserved Notation "[ l | m ] t"
-  (in custom stlc_tm at level 5, l custom stlc_tm at level 0,
-  t custom stlc_tm at next level, right associativity).
-Fixpoint subst (m : nat) (l : list tm) (t : tm) : tm :=
-  match t with
-  | tm_lvl n => nth n l n
-  | <{ t1 t2 }> => <{ [l|m]t1 [l|m]t2 }>
-  | <{ \: T, t1 }> => <{ \: T, [$(map (incr m) l) | m] t1 }>
-  | x => x
-  end
-where "[ l | m ] t" := (subst m l t) (in custom stlc_tm) : stlc_scope.
 
-(** Examples *)
-Compute <{ [[\: i, 1; $(tm_lvl 0)] | 1] \: o, 1 0 }>.
-Compute <{ [[\: i, 1; $(tm_lvl 0)] | 2] \: o, 1 0 }>.
-Compute <{ [[\: i, 0 1] | 2] \: o, 0 }>.
-Compute <{ [[\: i, 0 1] | 1] \: o, 0 }>.
-Compute <{ [[\: i, 0 0] | 0] \: o, 0 }>.
+  (********************)
+  (** ** Substitution *)
+  (********************)
 
-Compute <{ [[$(tm_lvl 0); \: i, 5; $(tm_lvl 2)] | 4] (1 2) }>.
-Compute <{ [[$(tm_lvl 0); \: i, 1 2] | 2] (\: o, 1) }>.
-Compute <{ [[$(tm_lvl 0); $(tm_lvl 1); \: i, 0 0] | 0] (\: o, \: i, 2 2) }>.
+  (** Increase the bound levels in a term by 1 *)
+  Fixpoint incr_bound m (t : tm) : tm :=
+    match t with
+    | tm_lvl n => tm_lvl (if Nat.leb m n then S n else n)
+    | tm_app t1 t2 => tm_app (incr_bound m t1) (incr_bound m t2)
+    | tm_abs T t1 => tm_abs T (incr_bound m t1)
+    | x => x
+    end.
+
+  Fixpoint subst m (l : list tm) (t : tm) : tm :=
+    match t with
+    | tm_lvl n => nth n l n
+    | tm_app s t => tm_app (subst m l s) (subst m l t)
+    | tm_abs T t => tm_abs T (subst m (map (incr_bound m) l) t)
+    | x => x
+    end.
+End Stlc.
